more changes

300 ANU Computing/Theoretical Computer Science/dafny/week10_tutorial.dfy
@@ -10,35 +10,95 @@ m = 1, a = 10, b = 5
 while m * b (1 * 5) <= a (10)
 increment m by one.
 
-2 * 5 (10) <= a (10), this is true, it doesn't exceed.
-m = 2
 
-3 * 5 (15) <= a (10), false, so m = 3
 
 Once we reach that state, we exit the while loop
 a = 10, b = 5, m = 3
 
-we perform m = m - 1, so m is now 2
+we perform m = m - 3, so m is now 2
 r = a - m * b = 10 - (2 * 5) = 10
 
-Answer = 2?
-
-ensures statement: 
-a == m * b + r, this should hold.
-0 <= r < b, 
+Answer = 2 r 0
 */
 
-method div(a: int, b: int) returns (m: int, r: int)
-  requires a >= 0 && b > 0
-  ensures a == m * b + r && 0 <= r < b
+// ensures statement explanation:
+// a == m * b + r holds because r is defined as a - m * b, just rearranged.
+// 0 <= r < b means the remainder must be non-negative and strictly less than b,
+// so that m is the largest integer where m * b <= a and no extra b fits into a.
+
+// method div(a: int, b: int) returns (m: int, r: int)
+//   requires a >= 0 && b > 0
+//   ensures a == m * b + r && 0 <= r < b
+// {
+//   m := 1;
+//   while (m * b <= a) 
+//   invariant (m - 1) * b <= a
+//   {
+//     m := m + 1;
+//   }
+//   m := m - 1;
+//   r := a - m * b;
+// }
+
+
+method bump_to_n(n: int) returns (i: int)
+  requires n >= 0
+  ensures i == n
 {
-  m := 1;
-  while (m * b <= a) 
-  invariant m >= 0
-  invariant a
+  i := 0;
+  while (i < n)
+    // TODO: invariant(s)
+    // TODO: decreases(...)
+    invariant i <= n
   {
-    m := m + 1;
+    i := i + 1;
   }
-  m := m - 1;
-  r := a - m * b;
 }
+
+
+method countdown(n: int) returns (z: int)
+  requires n >= 0
+  ensures z == 0
+{
+  var k := n;
+  while (k > 0)
+    // TODO: invariant(s)
+    // TODO: decreases(...)
+  {
+    k := k - 1;
+  }
+  z := k;
+}
+
+
+
+predicate dup_free(a: seq<int>)
+{
+  forall i,j :: 0 <= i < j < |a| ==> a[i] != a[j]
+}
+
+method nodup(a: seq<int>) returns (b: bool)
+  ensures b <==> dup_free(a)
+{
+  b := true;
+  var m := |a| - 1;
+
+  while (m > 0)
+    invariant dup_free(a) ==> b
+    invariant b ==> (forall p,q ::0 <= p < q < |a| && q > m ==> a[p] != a[q])
+  {
+    var n := m - 1;
+    while (n >= 0)
+      invariant dup_free(a) ==> b
+      invariant b ==> (forall p,q :: 0 <= p < q < |a| && q > m ==> a[p] != a[q])
+      invariant b ==> (forall p :: n < p < m ==> a[p] != a[m])
+    {
+      if a[n] == a[m] {
+        b := false;
+      }
+      n := n - 1;
+    }
+    m := m - 1;
+  }
+}
+
